src/Lib/BCT/BFL/Vst.v
@@ -1,0 +1,44 @@
+Require Import Core.Core Core.StructNormalizer VstLib.
+Require Import VST.floyd.proofauto.
+Require Import BFL.Exec.
+Require Import Clight.ber_tlv_length.
+
+Instance CompSpecs : compspecs. Proof. make_compspecs prog. Defined.
+Definition Vprog : varspecs. Proof. mk_varspecs prog. Defined.
+
+Section Ber_fetch_len.
+
+Definition ber_fetch_len_spec : ident * funspec :=
+  DECLARE _ber_fetch_length
+    WITH size : Z, data : list Z,
+         isc : Z, buf_b : block, buf_ofs : ptrofs, res_v : Z, res_ptr : val
+    PRE [tint, tptr tvoid, tuint, tptr tint]
+      PROP (isptr res_ptr;
+            Zlength data = size;
+            0 <= size <= Int.max_unsigned;
+            Int.signed (Int.repr size) <= Int.max_signed)
+      PARAMS (Vint (Int.repr isc); Vptr buf_b buf_ofs; Vint (Int.repr size); res_ptr)
+      GLOBALS ()
+      SEP (data_at Tsh (tarray tuchar (Zlength data)) 
+                   (map (fun v => Vubyte (Byte.repr v)) data) (Vptr buf_b buf_ofs);
+           data_at Tsh tuint (Vubyte (Byte.repr res_v)) res_ptr;
+           valid_pointer res_ptr)
+    POST [tint]
+      let r := ber_fetch_len data isc res_v size (sizeof tuint) 1 in
+      PROP ()
+      LOCAL (temp ret_temp (Vint (Int.repr (fst r))))
+      SEP (data_at Tsh (tarray tuchar (Zlength data)) 
+                   (map (fun v => Vubyte (Byte.repr v)) data) (Vptr buf_b buf_ofs);
+           data_at Tsh tuint (Vubyte (Byte.repr (snd r))) res_ptr;
+           valid_pointer res_ptr).
+
+Definition Gprog := ltac:(with_library prog [ber_fetch_len_spec]).
+
+Theorem ber_fetch_len : semax_body Vprog Gprog 
+                                          (normalize_function f_ber_fetch_length
+                                                              composites) 
+                                          ber_fetch_len_spec.
+Proof.
+Admitted.
+
+End Ber_fetch_len.
