src/Lib/BCT/BFT/Exec.v
@@ -1,0 +1,27 @@
+Require Import Core.Core Core.Notations Types.
+
+Fixpoint aux_loop (ptr : list Z) (val skip size tclass tag sizeofval : Z) := 
+  match ptr with
+  | oct :: xs => if skip <=? size
+                then if negb (oct & 128 =? 0)
+                     then let val' := (val << 7) or (oct & 127) in
+                          if negb (val >> (8 * sizeofval - 9) =? 0)
+                          then (-1, tag)
+                          else aux_loop xs val' (skip + 1) size tclass tag sizeofval
+                     else let val' := (val << 7) or oct in
+                         (skip, (val' << 2) or tclass)
+               else (0, tag)
+  | nil => (0, tag)
+  end.
+
+Definition bft_loop (ptr : list Z) (val size tclass tag sizeofval : Z) 
+  := aux_loop (skipn 1 ptr) val 2 size tclass tag sizeofval.
+
+Definition ber_fetch_tags (ptr : list Z) (val size tag sizeofval : Z) :=
+  if size =? 0
+  then (0, tag)
+  else let val := hd 0 ptr in 
+       let tclass := val >> 6 in 
+       if negb ((val & 31) =? 31)
+       then (1, ((val & 31) << 2) or tclass)
+       else bft_loop ptr 0 size tclass tag sizeofval.
