src/Lib/BCT/BFT/Vst.v
@@ -1,0 +1,48 @@
+Require Import Core.Core Core.StructNormalizer VstLib.
+Require Import VST.floyd.proofauto.
+Require Import BFT.Exec.
+Require Import Clight.ber_tlv_tag.
+
+Definition Vprog : varspecs. mk_varspecs prog. Defined.
+Instance CompSpecs : compspecs. make_compspecs prog. Defined.
+  
+Open Scope Z.
+
+Section Ber_fetch_tag.
+
+Definition ber_fetch_tag_spec : ident * funspec :=
+  DECLARE _ber_fetch_tag
+    WITH ptr_b : block, ptr_ofs : ptrofs, ptr_v : list Z, size : Z, 
+         tag_p : val
+    PRE [tptr tvoid, tuint, tptr tuint]
+      PROP (0 <= size <= Int.max_unsigned;
+            Zlength ptr_v = size;
+            Forall (fun x => 0 <= x <= Byte.max_unsigned) ptr_v;
+            Ptrofs.unsigned ptr_ofs + (Zlength ptr_v) < Ptrofs.modulus;
+           (* 0 <= tag_v <= Int.max_unsigned; *)
+            isptr tag_p)
+      PARAMS ((Vptr ptr_b ptr_ofs); Vint (Int.repr size); tag_p)
+      GLOBALS ()
+      SEP (data_at Tsh (tarray tuchar (Zlength ptr_v)) 
+                   (map Vubyte (map Byte.repr ptr_v)) (Vptr ptr_b ptr_ofs);
+           data_at_ Tsh tuint tag_p;
+           valid_pointer tag_p)
+    POST [tint]
+      let r := ber_fetch_tags ptr_v 0 size 0 (sizeof tuint) in
+      PROP ()
+      LOCAL (temp ret_temp (Vint (Int.repr (fst r))))
+      SEP (data_at Tsh (tarray tuchar (Zlength ptr_v)) 
+                   (map Vubyte (map Byte.repr ptr_v)) (Vptr ptr_b ptr_ofs);
+           data_at Tsh tuint (Vubyte (Byte.repr (snd r))) tag_p;
+           valid_pointer tag_p).
+
+Definition Gprog := ltac:(with_library prog [ber_fetch_tag_spec]).
+
+Theorem ber_fetch_tag : semax_body Vprog Gprog 
+                                   (normalize_function f_ber_fetch_tag composites) 
+                                   ber_fetch_tag_spec.
+Proof.
+Admitted.
+
+End Ber_fetch_tag.
+
